more small changes, notes

dnsprotect/small_changes_12-24/baseTest.dfy
@@ -70,4 +70,115 @@ abstract module LucidBase {
          ensures unchanged(this`queue)
          ensures forall i :: i >= e.time ==> stateInvariant (i)
   }
+
+   import opened ParseUtils
+   class Parser {
+      static ghost predicate validPacket(p:Packet) 
+      static ghost predicate parserSpecification(p : Packet, d : ParseDecision<Event>) 
+         requires validPacket(p)
+      static function parse(p : Packet) : ParseDecision<Event>
+         requires p.offset == 0
+         requires validPacket(p) 
+         ensures (parserSpecification(p, parse(p)))
+
+  }
+
+}
+
+
+module IntTypes {
+   // Integer types to use in executable code
+   type uint8 = x : nat | 0 <= x < 256
+   type uint16 = x : nat | 0 <= x < 65536
+   type uint20 = x : nat | 0 <= x < 1048576
+   type uint24 = x : nat | 0 <= x < 16777216
+   type uint32 = x : nat | 0 <= x < 4294967296
+   type uint48 = x : int | 0 <= x < 281474976710656
+}
+
+module ParseUtils {
+   // Utilities to use in the parser definition
+   import opened IntTypes
+   // A packet is a sequence of bytes, and a counter that 
+   // tracks how many bytes have been read from the packet
+   // up to this point.
+   datatype Packet = Packet(bytes : seq<uint8>, ghost offset : nat)
+   // A parser returns a decision on what to do with the packet
+   // either drop it, generate an event defined in the program, 
+   // or generate an event defined externally.
+   datatype ParseDecision<Event> = 
+      | Drop() 
+      | Generate(e:Event)
+      | GenerateExtern(name:string, args:seq<nat>)
+
+   // Parser helper functions
+   // skip n bytes from the packet
+   function skip(p : Packet, n : nat) : Packet
+      requires (|p.bytes| >= n)
+      ensures (skip(p, n).bytes == p.bytes[n..])
+   {
+      Packet(p.bytes[n..], p.offset + n)
+   }
+
+   // read 8 bits (1 byte) from the packet
+   function read8(p : Packet) : (Packet, uint8)
+      requires (|p.bytes| > 0)
+      ensures (read8(p).0.bytes == p.bytes[1..])
+   {
+      (Packet(p.bytes[1..], p.offset + 1), p.bytes[0])
+   }
+   function read16(p : Packet) : (Packet, uint16)
+      requires (|p.bytes| > 1)
+      ensures (read16(p).0.bytes == p.bytes[2..])
+   {
+      var out : uint16 := 0;
+      var out := out + (p.bytes[0] as uint16) * 256;
+      var out := out + (p.bytes[1] as uint16);
+      (Packet(p.bytes[2..], p.offset + 2), (p.bytes[0] as uint16) * 256 + (p.bytes[1] as uint16))
+   }
+   function read32(p : Packet) : (Packet, int)
+      requires (|p.bytes| > 3)
+      ensures (read32(p).0.bytes == p.bytes[4..])
+   {
+      var out : uint32 := 0;
+      var out := out + (p.bytes[0] as uint32) * 256 * 256 * 256;
+      var out := out + (p.bytes[1] as uint32) * 256 * 256;
+      var out := out + (p.bytes[2] as uint32) * 256;
+      var out := out + (p.bytes[3] as uint32);
+      (Packet(p.bytes[4..], p.offset + 4), out)
+   }
+   function read48(p : Packet) : (Packet, int)
+      requires (|p.bytes| > 5)
+      ensures (read48(p).0.bytes == p.bytes[6..])
+   {
+      var out : uint48 := 0;
+      var out := out + (p.bytes[0] as uint48) * 256 * 256 * 256 * 256 * 256;
+      var out := out + (p.bytes[1] as uint48) * 256 * 256 * 256 * 256;
+      var out := out + (p.bytes[2] as uint48) * 256 * 256 * 256;
+      var out := out + (p.bytes[3] as uint48) * 256 * 256;
+      var out := out + (p.bytes[4] as uint48) * 256;
+      var out := out + (p.bytes[5] as uint48);
+      (Packet(p.bytes[6..], p.offset + 6), out)
+   }
+
+   // the classic "network to host short" function
+   function ntohs(bs : seq<uint8>) : uint16
+      requires (|bs| == 2)
+   {
+      (bs[0] as uint16) * 256 + (bs[1] as uint16)
+   }
+   function htons(x : uint16) : seq<uint8>
+   {
+      [msb(x), lsb(x)]
+   }
+
+   function msb(x : uint16) : uint8
+   {
+      (x / 256) as uint8
+   }
+   function lsb(x : uint16) : uint8
+   {
+      (x % 256) as uint8
+   }
+
 }
